Challenge/Ripemd160/Submission/Proofs/Bytecode/KnownInputState.lean
@@ -120,7 +120,7 @@ def resultActiveWords (s : State) : UInt256 :=
 
 def resultState (s : State) (input : ByteArray) (i : Nat) : State :=
   { s with
-    pc := UInt256.ofNat 99
+    pc := UInt256.ofNat 107
     stack := [DriverTrace.blockOffsetWord i, Padding.paddedWord input]
     memory := resultMemory s.memory i
     activeWords := resultActiveWords s }
